theories_eval/LevelTwo.v
@@ -12,20 +12,25 @@ Definition mvar := nat.
 
 (** Quoted natural. *)
 Inductive qnat :=
-| Q_zero : qnat 
-| Q_succ : qnat -> qnat
-| Q_plus : qnat -> qnat -> qnat 
-| Q_ren : ren -> qnat -> qnat 
+(** Zero. *)
+| Q_zero : qnat
+(** Explicit renaming applied to a quoted natural. *)
+| Q_rapply : ren -> qnat -> qnat 
+(** Quoted natural meta-variable. *)
 | Q_mvar : mvar -> qnat
 
 (** Explicit renaming. *)
 with ren :=
-| R_shift : qnat -> ren
+(** Identity renaming. *)
+| R_id : ren
+(** Explicit shift. *)
+| R_shift : ren
+(** Renaming expansion. *)
 | R_cons : qnat -> ren -> ren
+(** Left to right composition of renamings. *)
 | R_comp : ren -> ren -> ren 
+(** Renaming meta-variable. *)
 | R_mvar : mvar -> ren.
-
-Notation "'Q_one'" := (Q_succ Q_zero).
 
 (*********************************************************************************)
 (** *** Expressions and explicit substitutions. *)
@@ -36,15 +41,16 @@ Reserved Notation "'term'" (at level 0).
 Reserved Notation "'arg' ty" (at level 0, ty at level 0).
 Reserved Notation "'args' tys" (at level 0, tys at level 0).
 
-(** Expressions over an abstract signature. 
-    Expressions are indexed by a kind: this is to avoid having too many 
-    distinct constructors for instantiation. *)
+(** Expressions are indexed by a kind: this is to avoid having too many 
+    distinct constructors for instantiation by a renaming/substitution. *)
 Inductive expr : kind -> Type :=
 
 (** Variable term constructor (de Bruijn index). *)
 | E_tvar : qnat -> term
 (** Non-variable term constructor, applied to a list of arguments. *)
 | E_tctor : forall c, args (ctor_type S.t c) -> term
+(** Term metavariable. We don't need argument or argument-list metavariables. *)
+| E_mvar : mvar -> term
 
 (** Empty argument list. *)
 | E_al_nil : args []
@@ -62,15 +68,15 @@ Inductive expr : kind -> Type :=
 | E_ren {k} : expr k -> ren -> expr k
 (** Instantiate an expressions with a substitution. *)
 | E_subst {k} : expr k -> subst -> expr k
-(** Term metavariable. We don't need argument or argument-list metavariables. *)
-| E_mvar : mvar -> term
 
 with subst :=
+(** Identity substitution. *)
+| S_id : subst
 (** Shift substitution. *)
-| S_shift : qnat -> subst
+| S_shift : subst
 (** Substitution expansion. *)
 | S_cons : term -> subst -> subst
-(** Substitution composition. *)
+(** Left to right composition of substitutions. *)
 | S_comp : subst -> subst -> subst
 (** View a renaming as a substitution. *)
 | S_ren : ren -> subst
@@ -80,33 +86,6 @@ with subst :=
 where "'term'" := (expr Kt)
   and "'arg' ty" := (expr (Ka ty))
   and "'args' tys" := (expr (Kal tys)).
-
-(** Notations for common expressions. *)
-
-(*Notation "'↑ᵣ' k" := (R_shift k) (at level 0, k at level 0).
-Notation "i '.ᵣ' r" := (R_cons i r) (at level 60, right associativity).
-Notation "r1 '>>ᵣ' r2" := (R_comp r1 r2) (at level 50, left associativity).
-
-Notation "'↑ₛ' k" := (E_sshift k) (at level 0, k at level 0).
-Notation "t '.ₛ' s" := (E_scons t s) (at level 60, right associativity).
-Notation "s1 '>>ₛ' s2" := (E_scomp s1 s2) (at level 50, left associativity).
-
-Notation "t '[ᵣ' s ']'" := (E_rinst t s) (at level 15, s at level 0, no associativity).
-Notation "t '[ₛ' s ']'" := (E_sinst t s) (at level 15, s at level 0, no associativity).*)
-
-(** The identity renaming. *)
-Notation "'rid'" := (R_shift Q_zero).
-
-(** The identity substitution. *)
-Notation "'sid'" := (S_shift Q_zero).
-
-(** Lift a renaming through a binder. *)
-(*Definition up_ren (r : ren) : ren :=
-  R_cons Q_zero (R_comp r (R_shift Q_one)).
-
-(** Lift a substitution through a binder. *)
-Definition up_subst (s : subst) : subst :=
-  S_cons (E_tvar Q_zero) (S_comp s (S_shift Q_one)).*)
 
 (*********************************************************************************)
 (** *** Evaluation. *)
@@ -124,13 +103,12 @@ Section Evaluation.
 
   Equations qeval : qnat -> nat :=
   qeval Q_zero := 0 ;
-  qeval (Q_succ i) := S (qeval i) ;
-  qeval (Q_plus x y) := qeval x + qeval y ;
-  qeval (Q_ren r i) := reval r (qeval i) ;
+  qeval (Q_rapply r i) := reval r (qeval i) ;
   qeval (Q_mvar x) := e.(assign_qnat) x
   
   with reval : ren -> O.ren :=
-  reval (R_shift i) := O.rshift (qeval i) ;
+  reval R_id := O.rid ;
+  reval R_shift := O.rshift ;
   reval (R_cons i r) := O.rcons (qeval i) (reval r) ;
   reval (R_comp r1 r2) := O.rcomp (reval r1) (reval r2) ;
   reval (R_mvar x) := e.(assign_ren) x.
@@ -148,7 +126,8 @@ Section Evaluation.
   eeval (E_mvar x) := e.(assign_term) x
   
   with seval : subst -> O.subst :=
-  seval (S_shift k) := O.sshift (qeval k) ;
+  seval S_id := O.sid ;
+  seval S_shift := O.sshift ;
   seval (S_cons t s) := O.scons (eeval t) (seval s) ;
   seval (S_comp s1 s2) := O.scomp (seval s1) (seval s2) ;
   seval (S_ren r) := O.rscomp (reval r) O.E_var ;
@@ -160,6 +139,8 @@ End Evaluation.
 (** *** Reification. *)
 (*********************************************************************************)
 
+(** Turn an Ltac2 [int] to a Rocq [nat]. 
+    Negative integers are mapped to [0]. *)
 Ltac2 rec nat_of_int (x : int) : constr := 
   if Int.le x 0 then constr:(0)
   else let y := nat_of_int (Int.sub x 1) in constr:(S $y).
@@ -198,20 +179,17 @@ Ltac2 add_subst_mvar (t : constr) (e : env) : env :=
   ; term_mvars := e.(term_mvars)
   ; subst_mvars := List.append (e.(subst_mvars)) [t] }.
 
+(* TODO: handle renamings directly applied to naturals. *)
 Ltac2 rec reify_nat (e : env) (t : constr) : env * constr := 
   lazy_match! t with 
   | 0 => e, constr:(Q_zero)
   | S ?i =>
     let (e, i) := reify_nat e i in 
-    e, constr:(Q_succ $i)
-  | ?x + ?y => 
-    let (e, x) := reify_nat e x in 
-    let (e, y) := reify_nat e y in 
-    e, constr:(Q_plus $x $y)
+    e, constr:(Q_rapply R_shift $i)
   | ?r ?i =>
     let (e, r) := reify_ren e r in
     let (e, i) := reify_nat e i in
-    e, constr:(Q_ren $r $i)
+    e, constr:(Q_rapply $r $i)
   | ?i => 
     let idx := nat_of_int (List.length (e.(qnat_mvars))) in
     let e := add_qnat_mvar i e in
@@ -220,9 +198,8 @@ Ltac2 rec reify_nat (e : env) (t : constr) : env * constr :=
 
 with reify_ren (e : env) (t : constr) : env * constr :=
   lazy_match! t with 
-  | O.rshift ?k =>
-    let (e, k) := reify_nat e k in 
-    e, constr:(R_shift $k) 
+  | O.rid => e, constr:(R_id)
+  | O.rshift => e, constr:(R_shift) 
   | O.rcons ?i ?r =>
     let (e, i) := reify_nat e i in 
     let (e, r) := reify_ren e r in 
@@ -273,10 +250,8 @@ Ltac2 rec reify_expr (e : env) (t : constr) : env * constr :=
 
 with reify_subst (e : env) (s : constr) : env * constr :=
   lazy_match! s with 
-  | O.sid => e, constr:(sid)
-  | O.sshift ?k => 
-    let (e, k) := reify_nat e k in 
-    e, constr:(S_shift $k)
+  | O.sid => e, constr:(S_id)
+  | O.sshift => e, constr:(S_shift)
   | O.scons ?t ?s =>
     let (e, t) := reify_expr e t in 
     let (e, s) := reify_subst e s in 
@@ -303,32 +278,28 @@ with reify_subst (e : env) (s : constr) : env * constr :=
 (** *** Discriminators. *)
 (*********************************************************************************)
 
-(** Normal forms and normalization functions need to distinguish terms based
-    on their head constructor(s). We provide discriminator functions which 
-    handle this, as well as a tactic [inv_discriminator]. *)
+(** Simplification needs to distinguish terms based on their head constructor(s). 
+    We provide discriminator functions which handle this, as well as 
+    tactics [inv_discriminator] and [solve_discriminators]. *)
 
-Definition is_qsucc x := exists x', x = Q_succ x'.
-Definition is_qplus x := exists y z, x = Q_plus y z.
-Definition is_qren x := exists r y, x = Q_ren r y.
+Definition is_qrapply x := exists r y, x = Q_rapply r y.
 Definition is_qmvar x := exists m, x = Q_mvar m.
 
-Definition is_rshift r := exists k, r = R_shift k.
 Definition is_rcons r := exists i r', r = R_cons i r'.
 Definition is_rcomp r := exists r1 r2 , r = R_comp r1 r2.
 Definition is_rmvar r := exists m, r = R_mvar m.
 
-Definition is_rshift_l r := exists k r2, r = R_comp (R_shift k) r2.
+Definition is_rid_l r := exists r2, r = R_comp R_id r2.
+Definition is_rshift_l r := exists r2, r = R_comp R_shift r2.
 Definition is_rcons_l r := exists i r' r2, r = R_comp (R_cons i r') r2.
 Definition is_rcomp_l r := exists r1 r2 r3, r = R_comp (R_comp r1 r2) r3.
 Definition is_rmvar_l r := exists m r2, r = R_comp (R_mvar m) r2.
 
-Definition is_sshift s := exists k, s = S_shift k.
 Definition is_scons s := exists t s', s = S_cons t s'.
 Definition is_scomp s := exists s1 s2 , s = S_comp s1 s2.
 Definition is_smvar s := exists m, s = S_mvar m.
 Definition is_sren s := exists r, s = S_ren r.
 
-Definition is_sshift_l s := exists k s2, s = S_comp (S_shift k) s2.
 Definition is_scons_l s := exists t s' s2, s = S_comp (S_cons t s') s2.
 Definition is_scomp_l s := exists s1 s2 s3, s = S_comp (S_comp s1 s2) s3.
 Definition is_smvar_l s := exists m s2, s = S_comp (S_mvar m) s2.
@@ -342,27 +313,24 @@ Ltac inv_discriminators :=
   solve [
     let H' := fresh "H" in
     repeat match goal with 
-    | [ H : is_qsucc _ |- _ ] => destruct H as (? & H') ; inv H'
-    | [ H : is_qren _ |- _ ] => destruct H as (? & ? & H') ; inv H'
+    | [ H : is_qrapply _ |- _ ] => destruct H as (? & ? & H') ; inv H'
     | [ H : is_qmvar _ |- _ ] => destruct H as (? & H') ; inv H'
 
-    | [ H : is_rshift _ |- _ ] => destruct H as (? & H') ; inv H'
     | [ H : is_rcons _ |- _ ] => destruct H as (? & ? & H') ; inv H'
     | [ H : is_rcomp _ |- _ ] => destruct H as (? & ? & H') ; inv H'
     | [ H : is_rmvar _ |- _ ] => destruct H as (? & H') ; inv H'
     
-    | [ H : is_rshift_l _ |- _ ] => destruct H as (? & ? & H') ; inv H'
+    | [ H : is_rid_l _ |- _ ] => destruct H as (? & H') ; inv H'
+    | [ H : is_rshift_l _ |- _ ] => destruct H as (? & H') ; inv H'
     | [ H : is_rcons_l _ |- _ ] => destruct H as (? & ? & ? & H') ; inv H'
     | [ H : is_rcomp_l _ |- _ ] => destruct H as (? & ? & ? & H') ; inv H'
     | [ H : is_rmvar_l _ |- _ ] => destruct H as (? & ? & H') ; inv H'
 
-    | [ H : is_sshift _ |- _ ] => destruct H as (? & H') ; inv H'
     | [ H : is_scons _ |- _ ] => destruct H as (? & ? & H') ; inv H'
     | [ H : is_scomp _ |- _ ] => destruct H as (? & ? & H') ; inv H'
     | [ H : is_smvar _ |- _ ] => destruct H as (? & H') ; inv H'
     | [ H : is_sren _ |- _ ] => destruct H as (? & H') ; inv H'
 
-    | [ H : is_sshift_l _ |- _ ] => destruct H as (? & ? & H') ; inv H'
     | [ H : is_scons_l _ |- _ ] => destruct H as (? & ? & ? & H') ; inv H'
     | [ H : is_scomp_l _ |- _ ] => destruct H as (? & ? & ? & H') ; inv H'
     | [ H : is_smvar_l _ |- _ ] => destruct H as (? & ? & H') ; inv H'
@@ -378,28 +346,24 @@ Ltac inv_discriminators :=
 Ltac solve_discriminators :=
   solve [
     match goal with 
-    | |- is_qsucc (Q_succ _) => repeat eexists
-    | |- is_qplus (Q_plus _ _) => repeat eexists
-    | |- is_qren (Q_ren _ _) => repeat eexists
+    | |- is_qrapply (Q_rapply _ _) => repeat eexists
     | |- is_qmvar (Q_mvar _) => repeat eexists
 
-    | |- is_rshift (R_shift _) => repeat eexists
     | |- is_rcons (R_cons _ _)  => repeat eexists
     | |- is_rcomp (R_comp _ _)  => repeat eexists
     | |- is_rmvar (R_mvar _)  => repeat eexists
 
-    | |- is_rshift_l (R_comp (R_shift _) _) => repeat eexists
+    | |- is_rid_l (R_comp R_id _) => repeat eexists
+    | |- is_rshift_l (R_comp R_shift _) => repeat eexists
     | |- is_rcons_l (R_comp (R_cons _ _) _) => repeat eexists
     | |- is_rcomp_l (R_comp (R_comp _ _) _) => repeat eexists
     | |- is_rmvar_l (R_comp (R_mvar _) _) => repeat eexists
 
-    | |- is_sshift (S_shift _) => repeat eexists
     | |- is_scons (S_cons _ _) => repeat eexists
     | |- is_scomp (S_comp _ _) => repeat eexists
     | |- is_smvar (S_mvar _) => repeat eexists
     | |- is_sren (S_ren _) => repeat eexists
 
-    | |- is_sshift_l (S_comp (S_shift _) _) => repeat eexists
     | |- is_scons_l (S_comp (S_cons _ _) _)  => repeat eexists
     | |- is_scomp_l (S_comp (S_comp _ _) _)  => repeat eexists
     | |- is_smvar_l (S_comp (S_mvar _) _)  => repeat eexists
@@ -409,120 +373,75 @@ Ltac solve_discriminators :=
 #[global] Hint Extern 3 => solve_discriminators : core.
 
 (*********************************************************************************)
-(** *** Renaming & naturals normal forms. *)
+(** *** Irreducible forms for renamings & naturals. *)
 (*********************************************************************************)
 
-(** Reducible quoted natural. *)
+(** Reducible quoted naturals. *)
 Inductive qred : qnat -> Prop :=
+
 (** Congruence. *)
-| QR_succ x : qred x -> qred (Q_succ x)
-| QR_plus x y : qred x \/ qred y -> qred (Q_plus x y)
-| QR_ren r x : rred r \/ qred x -> qred (Q_ren r x)
+| QR_ren r x : rred r \/ qred x -> qred (Q_rapply r x)
 
-(** Addition should pull out [Q_succ] from both arguments,
-    and by right associated. *)
-| QR_plus_zero_l x : qred (Q_plus x Q_zero)
-| QR_plus_zero_r x : qred (Q_plus Q_zero x)
-| QR_plus_plus_l x y z : qred (Q_plus (Q_plus x y) z)
-| QR_plus_succ_l x y : qred (Q_plus (Q_succ x) y)
-| QR_plus_succ_r x y : qred (Q_plus x (Q_succ y))
+| QR_ren_ren r1 r2 i : qred (Q_rapply r1 (Q_rapply r2 i))
+| QR_rcons_zero r : 
+    is_rcons r \/ is_rcons_l r -> qred (Q_rapply r Q_zero)
 
-(* Renamings should be fully applied to their argument.  *)
-| QR_ren_comp r1 r2 i : qred (Q_ren (R_comp r1 r2) i)
-| QR_ren_shift k i : qred (Q_ren (R_shift k) i)
-| QR_rcons_zero i r : qred (Q_ren (R_cons i r) Q_zero)
-| QR_rcons_succ i r k : qred (Q_ren (R_cons i r) (Q_succ k))
-
-(** Reducible renaming. *)
+(** Reducible renamings. *)
 with rred : ren -> Prop :=
+
 (** Congruence. *)
-| RR_shift k : qred k -> rred (R_shift k)
 | RR_cons i r : qred i \/ rred r -> rred (R_cons i r)
 | RR_comp r1 r2 : rred r1 \/ rred r2 -> rred (R_comp r1 r2)
 
-(** Composition should be right associated. *)
-| RR_rid_l r : rred (R_comp rid r)
-| RR_rid_r r : rred (R_comp r rid)
+(** Composition should be right associated, with neutral element [R_id]. *)
+| RR_rid_l r : rred (R_comp R_id r)
+| RR_rid_r r : rred (R_comp r R_id)
 | RR_comp_l r1 r2 r3 : rred (R_comp (R_comp r1 r2) r3)
 
-(** Renaming simplification. *)
 | RR_cons_l i r1 r2 : rred (R_comp (R_cons i r1) r2)
-| RR_shift_l k r : 
-  is_rshift r \/ is_rshift_l r -> rred (R_comp (R_shift k) r)
-| RR_shift_cons k r : 
-  is_rcons r -> rred (R_comp (R_shift (Q_succ k)) r).
+| RR_shift_cons r : 
+  is_rcons r \/ is_rcons_l r -> rred (R_comp R_shift r).
 
 Hint Constructors qred : core.
 Hint Constructors rred : core.
 
-(** Normal form quoted natural. *)
-Definition qnorm x := ~ qred x.
+(** Irreducible quoted natural. *)
+Definition qirred x := ~ qred x.
 
-(** Normal form renaming. *)
-Definition rnorm r := ~ rred r.
+(** Irreducible renaming. *)
+Definition rirred r := ~ rred r.
 
 (*********************************************************************************)
-(** *** Renaming & natural normal form properties. *)
+(** *** Properties of renaming & natural irreducible forms. *)
 (*********************************************************************************)
 
-Lemma qnorm_succ x :
-  qnorm (Q_succ x) <-> qnorm x.
+Lemma qirred_ren_mvar m i : 
+  qirred (Q_rapply (R_mvar m) i) <-> qirred i /\ ~is_qrapply i.
 Proof.
-split ; intros H H' ; apply H ; clear H.
-- now constructor.
-- now inv H'.
-Qed.
-
-Lemma qnorm_plus x y : 
-  qnorm (Q_plus x y) <-> 
-    qnorm x /\ qnorm y /\
-    x <> Q_zero /\ y <> Q_zero /\
-    ~is_qsucc x /\ ~is_qsucc y /\
-    ~is_qplus x.
-Proof.
-split.
-- intros H. split7 ; intros H' ; apply H ; clear H ; triv.
-  + subst. now constructor.
-  + subst. now constructor.
-  + destruct H' as (x' & ->). now constructor.
-  + destruct H' as (y' & ->). now constructor.
-  + destruct H' as (x1 & x2 & ->). now constructor.
-- intros (H1 & H2 & H3 & H4 & H5 & H6 & H7) H. inv H ; triv. now destruct H8.
-Qed.
-
-Lemma qnorm_ren_mvar m i : 
-  qnorm (Q_ren (R_mvar m) i) <-> qnorm i.
-Proof.
-split.
-- intros H H'. apply H ; clear H. constructor. now right.
-- intros H H'. inv H'. destruct H1 ; triv.
+split ; intros H.
+- split ; intros H' ; apply H ; clear H.
+  + constructor ; now right.
+  + destruct H' as (r & i' & ->). now constructor. 
+- intros H'. inv H'.
+  + destruct H1 ; triv.
+  + destruct H ; triv.
+  + destruct H1 ; triv.
 Qed.     
 
-Lemma qnorm_ren_cons i r k :
-  qnorm (Q_ren (R_cons i r) k) <->
-    qnorm i /\ rnorm r /\ qnorm k /\ k <> Q_zero /\ ~is_qsucc k.
+Lemma qirred_ren_cons i r k :
+  qirred (Q_rapply (R_cons i r) k) <-> qirred i /\ rirred r /\ is_qmvar k.
 Proof.
 split.
-- intros H. split5 ; intros H' ; apply H ; clear H.
-  + constructor ; left. constructor ; now left.  
-  + constructor ; left. constructor ; now right. 
-  + constructor ; now right.
-  + subst. now constructor.
-  + destruct H' as [k' ->]. now constructor.
-- intros (H1 & H2 & H3 & H4 & H5) H. inv H ; triv.
-  destruct H6 ; triv. inv H0. destruct H7 ; triv.
+- intros H. split3.
+  + intros H' ; apply H ; clear H. constructor ; left. constructor ; now left.
+  + intros H' ; apply H ; clear H. constructor ; left. constructor ; now right. 
+  + destruct k ; triv. 
+- intros (H1 & H2 & (? & ->)) H. inv H ; triv.
+  destruct H3 ; triv. inv H0. destruct H4 ; triv.
 Qed.
 
-Lemma rnorm_shift k : 
-  rnorm (R_shift k) <-> qnorm k.
-Proof. 
-split ; intros H H' ; apply H ; clear H.
-- now constructor.
-- now inv H'.
-Qed.
-
-Lemma rnorm_cons i r : 
-  rnorm (R_cons i r) <-> qnorm i /\ rnorm r.
+Lemma rirred_cons i r : 
+  rirred (R_cons i r) <-> qirred i /\ rirred r.
 Proof.
 split.
 - intros H. split ; intros H' ; apply H.
@@ -530,8 +449,8 @@ split.
 - intros [H1 H2] H. inv H. destruct H3 ; auto.
 Qed.
 
-Lemma rnorm_mvar_l m r : 
-  rnorm (R_comp (R_mvar m) r) <-> rnorm r /\ r <> rid.
+Lemma rirred_mvar_l m r : 
+  rirred (R_comp (R_mvar m) r) <-> rirred r /\ r <> R_id.
 Proof.
 split.
 - intros H. split.
@@ -540,91 +459,37 @@ split.
 - intros (H & H') H''. inv H'' ; triv. now destruct H1.
 Qed.      
 
-Lemma rnorm_shift_l k r : 
-  rnorm (R_comp (R_shift k) r) <-> 
-    qnorm k /\ 
-    rnorm r /\ 
-    k <> Q_zero /\ 
-    ~is_rshift r /\ 
-    ~is_rshift_l r /\
-    (is_qsucc k -> ~is_rcons r).
+Lemma rirred_shift_l r : 
+  rirred (R_comp R_shift r) <-> 
+    rirred r /\ r <> R_id /\ ~is_rcons r /\ ~is_rcons_l r.
 Proof.
 split.
-- intros H. split6 ; triv.
+- intros H. split4 ; triv.
   + intros H' ; apply H ; triv.
-  + intros H' ; apply H ; triv.
-  + intros H' ; apply H. subst ; triv.
-  + intros (k' & ->). intros H' ; triv.
-- intros (H1 & H2 & H3) H. inv H ; triv.
-  + destruct H4 ; auto. now inv H0.
-  + destruct H3 as (_ & ? & _) ; triv.
-  + destruct H3 as (_ & H3 & H3' & _). destruct H4 ; triv.
-  + destruct H4 as (? & ? & ->). destruct H3 as (_ & _ & _ & H3).
-    apply H3 ; triv.
+  + intros -> ; apply H. triv.
+- intros (H1 & H2) H. inv H ; triv.
+  + destruct H3 ; triv.
+  + destruct H3 ; triv.
 Qed.
+
+(*Lemma rirred_comp r1 r2 : 
+  rirred (R_comp r1 r2) <-> 
+    rirred r1 /\ rirred r2 /\ r2 <> R_id /\ (r1 = R_shift \/ is_rmvar r1).
+Proof.
+split.
+- intros H. split4.
+  + intros H' ; apply H. triv.
+  + intros H' ; apply H. triv.
+  + intros ->. triv.
+  + destruct r1 ; triv.
+- intros (H1 & H2 & H3 & [-> | (? & ->)]).
+  + rewrite rirred_shift_l. split4 ; triv.  *)
 
 (*********************************************************************************)
-(** *** Renaming & natural normalization. *)
+(** *** Simplification of renamings & quoted naturals. *)
 (*********************************************************************************)
 
-(** Add two normal form quoted naturals, where the left hand side
-    is neutral (i.e. is not Q_zero, Q_succ or Q_plus). *)
-Equations qplus_neutral : qnat -> qnat -> qnat :=
-qplus_neutral n Q_zero := n ;
-qplus_neutral n (Q_succ x) := Q_succ (qplus_neutral n x) ;
-qplus_neutral n x := Q_plus n x.
-
-Lemma qplus_neutral_sound e x y : 
-  qeval e (qplus_neutral x y) = qeval e x + qeval e y.
-Proof.
-funelim (qplus_neutral x y) ; simp qeval ; try lia.
-rewrite H. lia.
-Qed.
-#[global] Hint Rewrite qplus_neutral_sound : qeval.
-
-Lemma qplus_neutral_nf n x :
-  n <> Q_zero -> ~is_qsucc n -> ~is_qplus n -> qnorm n -> qnorm x -> qnorm (qplus_neutral n x).
-Proof.
-intros H1 H2 H3 H4 H5. funelim (qplus_neutral n x) ; clear Heqcall ; try easy.
-- rewrite qnorm_succ in *. now apply H.
-- rewrite qnorm_plus in *. split7 ; try easy.  
-  + now rewrite qnorm_plus.
-  + intros (k & Hk). inv Hk.
-- rewrite qnorm_plus. split7 ; try easy. intros (k & Hk). inv Hk.
-- rewrite qnorm_plus. split7 ; try easy. intros (k & Hk). inv Hk.
-Qed.  
-
-(** Add two normal form quoted naturals. *)
-Equations qplus : qnat -> qnat -> qnat :=
-qplus Q_zero y := y ;
-qplus (Q_succ x) y := Q_succ (qplus x y) ;
-qplus (Q_plus x y) z := qplus x (qplus y z) ;
-qplus x y := qplus_neutral x y.
-
-Lemma qplus_sound e x y :
-  qeval e (qplus x y) = qeval e x + qeval e y.
-Proof.
-funelim (qplus x y) ; simp qeval ; try lia.
-+ rewrite H. lia.
-+ rewrite H0, H. lia.
-Qed.  
-#[global] Hint Rewrite qplus_sound : qeval.
-
-Lemma qplus_nf x y : 
-  qnorm x -> qnorm y -> qnorm (qplus x y).
-Proof.
-intros H1 H2. funelim (qplus x y) ; clear Heqcall ; try easy.
-- rewrite qnorm_succ in *. now apply H.
-- rewrite qnorm_plus in H1. apply H0 ; try easy. now apply H.
-- apply qplus_neutral_nf ; try easy.
-  + intros (k & Hk) ; inv Hk.
-  + intros (x1 & x2 & H) ; inv H.
-- apply qplus_neutral_nf ; try easy.
-  + intros (k & Hk) ; inv Hk.
-  + intros (x1 & x2 & H) ; inv H.
-Qed.
-
-(** Helper function for [rdrop] which takes care of 
+(*(** Helper function for [rdrop] which takes care of 
     removing left composition by the identity. *)
 Equations do_rshift : qnat -> ren -> ren :=
 do_rshift Q_zero r := r ;
@@ -635,61 +500,45 @@ Lemma do_rshift_sound e k r :
 Proof. funelim (do_rshift k r) ; triv. Qed.
 #[global] Hint Rewrite do_rshift_sound : reval.
 
-Lemma do_rshift_nf k r :
-  qnorm k -> rnorm r -> (k <> Q_zero -> rnorm (R_comp (R_shift k) r)) -> rnorm (do_rshift k r).
-Proof. intros H1 H2 H3. funelim (do_rshift k r) ; triv ; now apply H3. Qed.
+Lemma do_rshift_irred k r :
+  qirred k -> rirred r -> (k <> Q_zero -> rirred (R_comp (R_shift k) r)) -> rirred (do_rshift k r).
+Proof. intros H1 H2 H3. funelim (do_rshift k r) ; triv ; now apply H3. Qed.*)
 
-(** Drop the [k] first elements in a normal form renaming [r]. *)
-Equations rdrop (k : qnat) (r : ren) : ren by struct r :=
-rdrop k (R_shift k') := R_shift (qplus k k') ;
-rdrop k (R_mvar m) := do_rshift k (R_mvar m) ;
-rdrop k (R_cons i r) with k => {
-  | Q_succ k' => rdrop k' r ;
-  | _ => do_rshift k (R_cons i r) } ;
-rdrop k (R_comp (R_shift k') r) := rdrop (qplus k k') r ;
-rdrop k r := do_rshift k r.
+(** Drop the first element in an irreducible renaming. *)
+Equations rtail (r : ren) : ren by struct r :=
+rtail R_id := R_shift ;
+rtail (R_cons _ r) := r ;
+rtail r := R_comp R_shift r.
 
-Lemma rdrop_sound e k r : 
-  reval e (rdrop k r) =₁ O.rcomp (O.rshift (qeval e k)) (reval e r).
+Lemma rtail_sound e r : 
+  reval e (rtail r) =₁ O.rcomp O.rshift (reval e r).
+Proof. funelim (rtail r) ; simp qeval ; triv. Qed.  
+#[global] Hint Rewrite rtail_sound : qeval reval.
+
+Lemma rtail_irred r : rirred r -> rirred (rtail r).
 Proof.
-funelim (rdrop k r) ; simp reval qeval ; triv.
-- now rewrite O.rshift_plus.
-- rewrite H. simp qeval. now rewrite <-O.rcomp_assoc, O.rshift_plus.
-Qed.
-#[global] Hint Rewrite rdrop_sound : reval qeval.
+intros H. funelim (rtail r) ; triv.
+- rewrite rirred_shift_l. split4 ; triv.
+- now rewrite rirred_cons in H.
+- rewrite rirred_shift_l. split4 ; triv.
+  intros (? & ? & ? & H1). inv H1. triv.
+- rewrite rirred_shift_l. split4 ; triv.
+Qed. 
 
-Lemma rdrop_nf k r : 
-  qnorm k -> rnorm r -> rnorm (rdrop k r).
-Proof.
-intros H1 H2. funelim (rdrop k r) ; triv.
-- rewrite rnorm_shift in *. now apply qplus_nf.
-- apply H.
-  + rewrite rnorm_shift_l in H2. now apply qplus_nf.
-  + now rewrite rnorm_shift_l in H2.
-- rewrite rnorm_mvar_l in H2. destruct H2 as [H2 H3]. 
-  apply do_rshift_nf ; triv.
-  + now rewrite rnorm_mvar_l.
-  + intros H. rewrite rnorm_shift_l. split6 ; triv.
-    rewrite rnorm_mvar_l ; triv.
-- apply do_rshift_nf ; triv. intros H3. rewrite rnorm_shift_l. split6 ; triv.
-- rewrite qnorm_succ in H1. rewrite rnorm_cons in H2. now apply H.
-- apply do_rshift_nf ; triv. intros _. rewrite rnorm_shift_l. split6 ; triv.
-- apply do_rshift_nf ; triv. intros _. rewrite rnorm_shift_l. split6 ; triv.
-- apply do_rshift_nf ; triv. intros _. rewrite rnorm_shift_l. split6 ; triv.
-Qed.
-
-(** Apply a normal form renaming to a normal form quoted natural. *)
+(** Apply an irreducible renaming to an irreducible quoted natural. *)
 Equations rapply (r : ren) (i : qnat) : qnat by struct r := 
+rapply R_id i := i ;
+rapply R_shift 
 rapply (R_shift k) i := qplus k i ;
-rapply (R_mvar m) r := Q_ren (R_mvar m) r ;
+rapply (R_mvar m) r := Q_rapply (R_mvar m) r ;
 rapply (R_cons i1 r) i with i => {
   | Q_zero := i1
   | Q_succ i' := rapply r i'
-  | _ := Q_ren (R_cons i1 r) i } ;
+  | _ := Q_rapply (R_cons i1 r) i } ;
 rapply (R_comp r1 r2) i with r1 => {
   | R_shift k := rapply r2 (qplus k i) ;
-  | R_mvar m := rapply r2 (Q_ren (R_mvar m) i)
-  | _ => (* This should not happen. *) Q_ren (R_comp r1 r2) i }.
+  | R_mvar m := rapply r2 (Q_rapply (R_mvar m) i)
+  | _ => (* This should not happen. *) Q_rapply (R_comp r1 r2) i }.
 
 Lemma rapply_sound e r i : 
   qeval e (rapply r i) = reval e r (qeval e i).
@@ -699,19 +548,19 @@ rewrite H. simp qeval. reflexivity.
 Qed.
 #[global] Hint Rewrite rapply_sound : qeval.
 
-Lemma rapply_nf r i : 
-  rnorm r -> qnorm i -> qnorm (rapply r i).
+Lemma rapply_irred r i : 
+  rirred r -> qirred i -> qirred (rapply r i).
 Proof. 
 intros H1 H2. funelim (rapply r i) ; triv.
-- rewrite rnorm_shift in H1. now apply qplus_nf.
-- now rewrite qnorm_ren_mvar.
-- now rewrite rnorm_cons in H1.
-- rewrite rnorm_cons in H1. rewrite qnorm_succ in H2. now apply H.
-- rewrite qnorm_ren_cons. rewrite rnorm_cons in H1. split5 ; triv.
-- rewrite qnorm_ren_cons. rewrite rnorm_cons in H1. split5 ; triv.
-- rewrite qnorm_ren_cons. rewrite rnorm_cons in H1. split5 ; triv.
-- rewrite rnorm_shift_l in H1. apply H ; triv. now apply qplus_nf.
-- rewrite rnorm_mvar_l in H1. apply H ; triv. now rewrite qnorm_ren_mvar.
+- rewrite rirred_shift in H1. now apply qplus_irred.
+- now rewrite qirred_ren_mvar.
+- now rewrite rirred_cons in H1.
+- rewrite rirred_cons in H1. rewrite qirred_succ in H2. now apply H.
+- rewrite qirred_ren_cons. rewrite rirred_cons in H1. split5 ; triv.
+- rewrite qirred_ren_cons. rewrite rirred_cons in H1. split5 ; triv.
+- rewrite qirred_ren_cons. rewrite rirred_cons in H1. split5 ; triv.
+- rewrite rirred_shift_l in H1. apply H ; triv. now apply qplus_irred.
+- rewrite rirred_mvar_l in H1. apply H ; triv. now rewrite qirred_ren_mvar.
 Qed.   
 
 (** Helper function for [rcomp] which takes care of 
@@ -725,14 +574,14 @@ Lemma rcomp_aux_sound e r1 r2 :
 Proof. funelim (rcomp_aux r1 r2) ; simp qeval ; triv. Qed.
 #[global] Hint Rewrite rcomp_aux_sound : qeval reval. 
 
-Lemma rcomp_aux_nf r1 r2 :
-  rnorm r1 -> rnorm r2 -> (r2 <> rid -> rnorm (R_comp r1 r2)) -> rnorm (rcomp_aux r1 r2).
+Lemma rcomp_aux_irred r1 r2 :
+  rirred r1 -> rirred r2 -> (r2 <> rid -> rirred (R_comp r1 r2)) -> rirred (rcomp_aux r1 r2).
 Proof. 
 intros H1 H2 H3. funelim (rcomp_aux r1 r2) ; triv.
 all: apply H3 ; intros H ; inv H.
 Qed.  
 
-(** Compose two normal form renamings. *)
+(** Compose two irreducible renamings. *)
 Equations rcomp (r1 r2 : ren) : ren by struct r1 :=
 rcomp (R_shift k) r := rdrop k r ;
 rcomp (R_cons i r1) r2 := R_cons (rapply r2 i) (rcomp r1 r2) ;
@@ -752,41 +601,41 @@ funelim (rcomp r1 r2) ; simp reval qeval ; triv.
 Qed.  
 #[global] Hint Rewrite rcomp_sound : reval qeval.
 
-Lemma rcomp_nf r1 r2 : 
-  rnorm r1 -> rnorm r2 -> rnorm (rcomp r1 r2).
+Lemma rcomp_irred r1 r2 : 
+  rirred r1 -> rirred r2 -> rirred (rcomp r1 r2).
 Proof.
 intros H1 H2. funelim (rcomp r1 r2) ; triv.
-- rewrite rnorm_shift in H1. now apply rdrop_nf.
-- rewrite rnorm_cons in * ; split.
-  + now apply rapply_nf.
+- rewrite rirred_shift in H1. now apply rdrop_irred.
+- rewrite rirred_cons in * ; split.
+  + now apply rapply_irred.
   + now apply H.
-- apply rcomp_aux_nf ; triv. intros H. now rewrite rnorm_mvar_l.
-- rewrite rnorm_shift_l in H1. apply rdrop_nf ; triv. now apply H.
-- rewrite rnorm_mvar_l in H1. apply rcomp_aux_nf ; triv.  
+- apply rcomp_aux_irred ; triv. intros H. now rewrite rirred_mvar_l.
+- rewrite rirred_shift_l in H1. apply rdrop_irred ; triv. now apply H.
+- rewrite rirred_mvar_l in H1. apply rcomp_aux_irred ; triv.  
   + now apply H.
-  + intros H3. rewrite rnorm_mvar_l. split ; triv. apply H ; triv.
+  + intros H3. rewrite rirred_mvar_l. split ; triv. apply H ; triv.
 Qed.
 
-(** Normalize a quoted natural. *)
-Equations qnormalize : qnat -> qnat :=
-qnormalize Q_zero := Q_zero ;
-qnormalize (Q_succ i) := Q_succ (qnormalize i) ;
-qnormalize (Q_plus x y) := qplus (qnormalize x) (qnormalize y) ;
-qnormalize (Q_ren r i) := rapply (rnormalize r) (qnormalize i) ;
-qnormalize (Q_mvar m) := Q_mvar m 
+(** Simplify a quoted natural. *)
+Equations qsimp : qnat -> qnat :=
+qsimp Q_zero := Q_zero ;
+qsimp (Q_succ i) := Q_succ (qsimp i) ;
+qsimp (Q_plus x y) := qplus (qsimp x) (qsimp y) ;
+qsimp (Q_rapply r i) := rapply (rsimp r) (qsimp i) ;
+qsimp (Q_mvar m) := Q_mvar m 
 
-(** Normalize a renaming. *)
-with rnormalize : ren -> ren :=
-rnormalize (R_shift k) := R_shift (qnormalize k) ;
-rnormalize (R_cons i r) := R_cons (qnormalize i) (rnormalize r) ;
-rnormalize (R_comp r1 r2) := rcomp (rnormalize r1) (rnormalize r2) ;
-rnormalize (R_mvar m) := R_mvar m.
+(** Simplify a renaming. *)
+with rsimp : ren -> ren :=
+rsimp (R_shift k) := R_shift (qsimp k) ;
+rsimp (R_cons i r) := R_cons (qsimp i) (rsimp r) ;
+rsimp (R_comp r1 r2) := rcomp (rsimp r1) (rsimp r2) ;
+rsimp (R_mvar m) := R_mvar m.
 
-Lemma qrnormalize_sound_aux e :
-  (forall i, qeval e (qnormalize i) = qeval e i) *
-  (forall r, reval e (rnormalize r) =₁ reval e r).
+Lemma qrsimp_sound_aux e :
+  (forall i, qeval e (qsimp i) = qeval e i) *
+  (forall r, reval e (rsimp r) =₁ reval e r).
 Proof. 
-apply qnormalize_elim with 
+apply qsimp_elim with 
   (P := fun i res => qeval e res = qeval e i)
   (P0 := fun r res => reval e res =₁ reval e r).
 all: intros ; simp qeval reval ; triv.
@@ -796,35 +645,35 @@ all: intros ; simp qeval reval ; triv.
 - now rewrite H, H0.
 Qed.    
 
-Lemma qnormalize_sound e i : qeval e (qnormalize i) = qeval e i.
-Proof. now apply qrnormalize_sound_aux. Qed.
-#[global] Hint Rewrite qnormalize_sound : qeval.
+Lemma qsimp_sound e i : qeval e (qsimp i) = qeval e i.
+Proof. now apply qrsimp_sound_aux. Qed.
+#[global] Hint Rewrite qsimp_sound : qeval.
 
-Lemma rnormalize_sound e r : reval e (rnormalize r) =₁ reval e r.
-Proof. now apply qrnormalize_sound_aux. Qed.
-#[global] Hint Rewrite rnormalize_sound : qeval reval.
+Lemma rsimp_sound e r : reval e (rsimp r) =₁ reval e r.
+Proof. now apply qrsimp_sound_aux. Qed.
+#[global] Hint Rewrite rsimp_sound : qeval reval.
 
-Lemma qrnormalize_nf_aux : 
-  (forall i, qnorm (qnormalize i)) * (forall r, rnorm (rnormalize r)).
+Lemma qrsimp_irred_aux : 
+  (forall i, qirred (qsimp i)) * (forall r, rirred (rsimp r)).
 Proof.
-apply qnormalize_elim with (P := fun _ res => qnorm res) (P0 := fun _ res => rnorm res).
+apply qsimp_elim with (P := fun _ res => qirred res) (P0 := fun _ res => rirred res).
 all: intros ; triv.
-- now rewrite qnorm_succ.
-- now apply qplus_nf.
-- now apply rapply_nf.
-- now rewrite rnorm_shift.
-- now rewrite rnorm_cons.
-- now apply rcomp_nf.
+- now rewrite qirred_succ.
+- now apply qplus_irred.
+- now apply rapply_irred.
+- now rewrite rirred_shift.
+- now rewrite rirred_cons.
+- now apply rcomp_irred.
 Qed.
 
-Lemma qnormalize_nf i : qnorm (qnormalize i).
-Proof. now apply qrnormalize_nf_aux. Qed.
+Lemma qsimp_irred i : qirred (qsimp i).
+Proof. now apply qrsimp_irred_aux. Qed.
 
-Lemma rnormalize_nf r : rnorm (rnormalize r).
-Proof. now apply qrnormalize_nf_aux. Qed.
+Lemma rsimp_irred r : rirred (rsimp r).
+Proof. now apply qrsimp_irred_aux. Qed.
   
 (*********************************************************************************)
-(** *** Substitutions & expressions normal forms. *)
+(** *** Irreducible forms for substitutions & expressions. *)
 (*********************************************************************************)
 
 (** Expressions in which we can push renamings/substitutions. *)
@@ -859,12 +708,13 @@ Inductive ered : forall {k}, expr k -> Prop :=
     is_scons s \/ is_scons_l s -> ered (E_subst (E_tvar Q_zero) s)
 | ER_scons_succ s i : 
    is_scons s \/ is_scons_l s -> ered (E_subst (E_tvar (Q_succ i)) s)
+| ER_sren_var s i : 
+   is_sren s \/ is_sren_l s -> ered (E_subst (E_tvar i) s)
 
-(** Miscellaneous simplifications. *)
-| ER_ren_rid {k} (e : expr k) : ered (E_ren e rid)
-| ER_subst_sid {k} (e : expr k) : ered (E_subst e sid)
-| ER_sren {k} (e : expr k) s : 
-  is_sren s \/ is_sren_l s -> ered (E_subst e s)
+(** Apply a substitution/renaming to a meta-variable. *)
+| ER_ren_rid (m : mvar) : ered (E_ren (E_mvar m) rid)
+| ER_subst_sid (m : mvar ) : ered (E_subst (E_mvar m) sid)
+| ER_ren_mvar (m : mvar) r : ered (E_subst (E_mvar m) (S_ren r))
 
 (** Reducible substitutions. *)
 with sred : subst -> Prop :=
@@ -875,44 +725,44 @@ with sred : subst -> Prop :=
 | SR_comp s1 s2 : sred s1 \/ sred s2 -> sred (S_comp s1 s2)
 | SR_ren r : rred r -> sred (S_ren r)
 
-(** Composition should be right associated. *)
+(** Composition should be right associated, with neutral element [sid]. *)
 | SR_sid_l s : sred (S_comp sid s)
 | SR_sid_r s : sred (S_comp s sid)
 | SR_comp_l s1 s2 s3: sred (S_comp (S_comp s1 s2) s3)
 
-(** Composition left-distributes over [S_ren] and [S_cons]. 
-    In particular, in [S_ren r >> s], we enforce that [r] is a meta-variable. *)
-| SR_ren_l r s : ~is_rmvar r -> sred (S_comp (S_ren r) s)
+(** Push [S_ren] into renamings. *)
+| SR_ren_distrib r : ~is_rmvar r -> sred (S_ren r)
+(** Composition distributes over [S_cons]. *)
 | SR_cons_l t s1 s2 : sred (S_comp (S_cons t s1) s2)
-
-(** Miscellaneous substitution simplifications. *)
+(** Combine successive shifts. *)
 | SR_shift_l k s : 
   is_sshift s \/ is_sshift_l s -> sred (S_comp (S_shift k) s)
-| SR_shift_cons k t s : 
-  sred (S_comp (S_shift (Q_succ k)) (S_cons t s)).
+(** Simplify [shift >> (t . s)] into [s]. *)
+| SR_shift_cons k s : 
+  is_scons s \/ is_scons_l s -> sred (S_comp (S_shift (Q_succ k)) s).
 
 Hint Constructors ered : core.
 Hint Constructors sred : core.
 
-(** Normal form expression. *)
-Definition enorm {k} (e : expr k) := ~ered e.
+(** Irreducible expression. *)
+Definition eirred {k} (e : expr k) := ~ered e.
 
-(** Normal form substitution. *)
-Definition snorm s := ~sred s.
+(** Irreducible substitution. *)
+Definition sirred s := ~sred s.
 
 (*********************************************************************************)
-(** *** Substitution & expression normal form properties. *)
+(** *** Properties of substitution & expression irreducible forms. *)
 (*********************************************************************************)
 
-Lemma snorm_shift k : snorm (S_shift k) <-> qnorm k.
+Lemma sirred_shift k : sirred (S_shift k) <-> qirred k.
 Proof.
 split ; intros H H' ; apply H ; clear H.
 - now constructor.
 - now inv H'.
 Qed.
 
-Lemma snorm_cons t s : 
-  snorm (S_cons t s) <-> enorm t /\ snorm s.
+Lemma sirred_cons t s : 
+  sirred (S_cons t s) <-> eirred t /\ sirred s.
 Proof.
 split ; intros H.
 - split ; intros H' ; apply H ; clear H.
@@ -921,10 +771,10 @@ split ; intros H.
 - intros H'. inv H'. destruct H1 ; triv.
 Qed.   
 
-Lemma snorm_shift_l k s : 
-  snorm (S_comp (S_shift k) s) <->
-    qnorm k /\ 
-    snorm s /\ 
+Lemma sirred_shift_l k s : 
+  sirred (S_comp (S_shift k) s) <->
+    qirred k /\ 
+    sirred s /\ 
     k <> Q_zero /\
     ~is_sshift s /\ 
     ~is_sshift_l s /\
@@ -937,16 +787,16 @@ split.
   + subst. now constructor.
   + destruct H' as [k' ->]. apply SR_shift_l. triv.
   + destruct H' as (k' & r' & ->). apply SR_shift_l ; triv. 
-  + destruct H' as [(k' & ->) (i & r' & ->)]. now constructor.   
+  + destruct H' as [(k' & ->) (i & r' & ->)]. apply SR_shift_cons. left. triv.
 - intros (H1 & H2 & H3) H. inv H ; try easy.
   + destruct H4 ; auto. now inv H0.
   + destruct H3 as (_ & H3 & _) ; apply H3. triv.
   + destruct H3 as (_ & H3 & H3' & _) ; apply H3. now destruct H4.
-  + destruct H3 as (_ & _ & _ & H3) ; apply H3. triv.
-Qed. 
+  + destruct H3 as (_ & _ & _ & H3) ; apply H3.
+Admitted.
 
-Lemma snorm_ren_l r s : 
-  snorm (S_comp (S_ren r) s) <-> is_rmvar r /\ snorm s /\ s <> sid.
+(*Lemma sirred_ren_l r s : 
+  sirred (S_comp (S_ren r) s) <-> is_rmvar r /\ sirred s /\ s <> sid.
 Proof.
 split ; intros H.
 - split3.
@@ -959,8 +809,8 @@ split ; intros H.
   destruct H as ((m & ->) & _ & _). inv H2.
 Qed.
 
-Lemma snorm_mvar_l m s : 
-  snorm (S_comp (S_mvar m) s) <-> snorm s /\ s <> sid.
+Lemma sirred_mvar_l m s : 
+  sirred (S_comp (S_mvar m) s) <-> sirred s /\ s <> sid.
 Proof.
 split.
 - intros H. split.
@@ -969,15 +819,15 @@ split.
 - intros (H & H') H''. inv H'' ; triv. now destruct H1.
 Qed. 
 
-Lemma snorm_ren r : snorm (S_ren r) <-> rnorm r.
+Lemma sirred_ren r : sirred (S_ren r) <-> rirred r.
 Proof.
 split ; intros H H' ; apply H ; clear H.
 - now constructor.
 - now inv H'.
-Qed.  
+Qed.  *)
 
 (*********************************************************************************)
-(** *** Substitution & expressions normalization. *)
+(** *** Simplify substitutions & expressions. *)
 (*********************************************************************************)
 
 (** Helper function for [sdrop] which takes care of 
@@ -991,11 +841,11 @@ Lemma do_sshift_sound e k s :
 Proof. funelim (do_sshift k s) ; triv. Qed.
 #[global] Hint Rewrite do_sshift_sound : seval.
 
-Lemma do_sshift_nf k s :
-  qnorm k -> snorm s -> (k <> Q_zero -> snorm (S_comp (S_shift k) s)) -> snorm (do_sshift k s).
+Lemma do_sshift_irred k s :
+  qirred k -> sirred s -> (k <> Q_zero -> sirred (S_comp (S_shift k) s)) -> sirred (do_sshift k s).
 Proof. intros H1 H2 H3. funelim (do_sshift k s) ; triv ; now apply H3. Qed.
 
-(** Drop the [k] first elements in a normal form substitution [s]. *)
+(** Drop the [k] first elements in an irreducible substitution [s]. *)
 Equations sdrop (k : qnat) (s : subst) : subst by struct s :=
 sdrop k (S_shift k') := S_shift (qplus k k') ;
 sdrop k (S_cons t s) with k := {
@@ -1014,17 +864,35 @@ funelim (sdrop k s) ; simp seval eeval qeval ; triv.
 Qed.
 #[global] Hint Rewrite sdrop_sound : seval eeval.   
 
-Lemma sdrop_nf k s :
-  qnorm k -> snorm s -> snorm (sdrop k s).
+Lemma sdrop_irred k s :
+  qirred k -> sirred s -> sirred (sdrop k s).
 Proof.
 intros H1 H2. funelim (sdrop k s) ; triv.
-all: try solve [ apply do_sshift_nf ; triv ; [] ; intros H3 ; rewrite snorm_shift_l ;
+all: try solve [ apply do_sshift_irred ; triv ; [] ; intros H3 ; rewrite sirred_shift_l ;
   split6 ; triv ; [] ; intros (? & ?) ; triv ].
-- rewrite snorm_shift in *. now apply qplus_nf.
-- rewrite snorm_shift_l in H2. apply H ; triv. now apply qplus_nf.
-- rewrite snorm_ren in *. now apply rdrop_nf.
-- rewrite qnorm_succ in H1. rewrite snorm_cons in H2. now apply H.
+- rewrite sirred_shift in *. now apply qplus_irred.
+- rewrite sirred_shift_l in H2. apply H ; triv. now apply qplus_irred.
+- rewrite sirred_ren in *. now apply rdrop_irred.
+- rewrite qirred_succ in H1. rewrite sirred_cons in H2. now apply H.
 Qed.
+
+(** Apply an irreducible substitution to an irreducible natural. *)
+Equations sapply (s : subst) (i : qnat) : term by struct s := 
+sapply (S_shift k) i := E_tvar (qplus k i) ;
+sapply (S_comp (S_shift k) s) i := sapply s (qplus k i) ;
+
+sapply (S_cons t s) Q_zero := t ;
+sapply (S_comp (S_cons t s1) s2) Q_zero := t ;
+
+sapply (S_cons t s) (Q_succ i) := sapply s i ;
+sapply (S_comp (S_cons t s1) s2) (Q_succ i) := sapply s2 (sapply s1 i) ;
+
+sapply (S_ren r) i := E_tvar (rapply r i) ;
+sapply (S_comp (S_ren r) s) i := sapply s (rapply r i) ;
+
+sapply s i with i := { 
+  | Q_rapply (R_cons i0 r0) i' => E_subst (S_cons (sapply s i0) (rscomp r0 s)) i'
+  | _ => E_subst (E_tvar i) s }.
 
 End Make.
 
@@ -1090,7 +958,7 @@ Ltac2 test_tac () : unit :=
     let e := build_env e in
     printf "ENV %t" e ;
     change (qeval $e $l' = $r) ;
-    rewrite <-(qnormalize_sound $e $l')
+    rewrite <-(qsimp_sound $e $l')
   | _ => Control.throw_invalid_argument "not an equality on naturals"
   end.
 
@@ -1098,7 +966,7 @@ Lemma test : left = right.
 Proof.
 unfold left, right.
 ltac2:(test_tac ()).
-cbv [qnormalize qnormalize_functional rnormalize_functional qplus qplus_neutral rapply
+cbv [qsimp qsimp_functional rsimp_functional qplus qplus_neutral rapply
      rapply_clause_3 rapply_clause_4].
 cbv [qeval reval qeval_functional reval_functional 
      assign_ren assign_qnat nth].
